Add simple addition extraction test

code/experimental/he/Hacl.Test.HE.fst
@@ -1,17 +1,62 @@
 module Hacl.Test.HE
 
-open FStar.HyperStack.All
+open C.Failure
+open FStar.HyperStack
+open FStar.HyperStack.ST
 open FStar.Mul
-
-open LowStar.Buffer
 
 open Lib.IntTypes
 open Lib.Buffer
-open Lib.PrintBuffer
 
+open Hacl.Impl.HE.GM
+open Hacl.Impl.Comparison
+open Hacl.Impl.Addition
+
+
+inline_for_extraction unfold noextract
+let print_str x = C.String.print (C.String.of_literal x)
+
+inline_for_extraction unfold noextract
+let print_strln x = print_str (x ^ "\n")
+
+inline_for_extraction unfold noextract
+val print_bool: b:bool -> St unit
+let print_bool b =
+  C.String.print (if b then C.String.of_literal "true\n" else C.String.of_literal "false\n")
+
+inline_for_extraction unfold noextract
+val toBuffer:
+    size:size_t ->
+    l:list uint64 ->
+    Stack (lbuffer uint64 size) (requires fun h -> true) (ensures fun h0 b h1 -> live h1 b)
+let toBuffer size l =
+  admit();
+  createL (normalize_term l)
+
+val test1: unit -> St unit
+let test1 _ =
+  let list1 =
+    toBuffer 16ul (normalize_term (List.Tot.map u64
+      [0xa5; 0x6e; 0x4a; 0x0e; 0x70; 0x10; 0x17; 0x58; 0x9a; 0x51; 0x87; 0xdc; 0x7e; 0xa8; 0x41; 0xd1]))
+      in
+
+  let list2 =
+    toBuffer 16ul (normalize_term (List.Tot.map u64
+      [0x00; 0x11; 0x22; 0x33; 0x44; 0x55; 0x66; 0x77; 0x9a; 0x51; 0x87; 0xdc; 0x7e; 0xa8; 0x41; 0xd1]))
+      in
+
+  let list3 =
+    toBuffer 16ul (normalize_term (List.Tot.map u64
+      [0x00; 0x00; 0x00; 0x00; 0x00; 0x00; 0x00; 0x00; 0x00; 0x00; 0x00; 0x00; 0x00; 0x00; 0x00; 0x00]))
+      in
+
+  let _ = bn_add 16ul list1 16ul list2 list3 in
+  let res = bn_is_less 16ul list1 16ul list3 in
+  print_bool res
 
 val main: unit -> St C.exit_code
 let main () =
-  C.String.print
-    (C.String.of_literal "\n\n ====== No argmax tests are written yet ====== \n\n\n");
+  print_strln "\n ====== Sample: ====== \n";
+  test1 ();
+  print_strln "\n ===================== \n";
   C.EXIT_SUCCESS
